{-# OPTIONS --safe --lossy-unification #-}
module Cubical.Categories.Profunctor.General where

open import Cubical.Reflection.RecordEquiv

open import Cubical.Foundations.Prelude
open import Cubical.Foundations.HLevels
open import Cubical.Foundations.Isomorphism
open import Cubical.Foundations.Equiv
open import Cubical.Foundations.Structure
open import Cubical.Foundations.Univalence
open import Cubical.Foundations.Function renaming (_∘_ to _∘f_)

open import Cubical.Categories.Category renaming (isIso to isIsoC)
open import Cubical.Categories.Functor
open import Cubical.Categories.Bifunctor.Redundant
open import Cubical.Categories.Instances.Functors
open import Cubical.Categories.NaturalTransformation
open import Cubical.Categories.NaturalTransformation.More
open import Cubical.Categories.NaturalTransformation.Base
open import Cubical.Categories.Constructions.BinProduct
open import Cubical.Categories.Constructions.BinProduct.More
open import Cubical.Categories.Instances.Sets
open import Cubical.Categories.Instances.Sets.More
open import Cubical.Categories.Functors.Constant
open import Cubical.Categories.Functors.More
open import Cubical.Categories.Functors.HomFunctor
open import Cubical.Data.Sigma

open import Cubical.Categories.Presheaf.Representable
open import Cubical.Categories.Presheaf.More
open import Cubical.Categories.Instances.Functors.More

private
  variable
    ℓC ℓC' ℓD ℓD' ℓS ℓR : Level

open Category
open Functor
open UniversalElement
open Bifunctor

-- Convenient notation for function composition in the same order as
-- ⋆⟨ C ⟩ in a category C
-- i.e. for ⋆⟨ SET _ ⟩ without having to prove that everything indeed lives
-- SET _.
_⋆f_ : {ℓ : Level} {A : Type ℓ } → {B : A → Type ℓ} →
       {C : (a : A) → B a → Type ℓ} →
       (f : (a : A) → B a) → (g : {a : A} → (b : B a) → C a b) →
       (a : A) → C a (f a)
f ⋆f g = λ x → (g ∘f f) x

_o-[_]-*_ : (C : Category ℓC ℓC') → ∀ ℓS → (D : Category ℓD ℓD') → Type _
C o-[ ℓS ]-* D = Bifunctor (C ^op) D (SET ℓS)

_*-[_]-o_ : (C : Category ℓC ℓC') → ∀ ℓS → (D : Category ℓD ℓD') → Type _
C *-[ ℓS ]-o D = D o-[ ℓS ]-* C

module _  {C : Category ℓC ℓC'}
          {D : Category ℓD ℓD'}
          (R : C o-[ ℓR ]-* D) (S : C o-[ ℓS ]-* D) where

  private
    ℓmaxCDSR : Level
    ℓmaxCDSR = (ℓ-max ℓC (ℓ-max ℓC' (ℓ-max ℓD (ℓ-max ℓD' (ℓ-max ℓS ℓR)))))

  -- A definition of profunctor homomorphism that avoids Lifts
  record ProfHomo : Type ℓmaxCDSR where
    field
      PH-ob : ∀ {c d} → (r : ⟨ R ⟅ c , d ⟆b ⟩) → ⟨ S ⟅ c , d ⟆b ⟩
      PH-natL : ∀ {c c' d} (f : C [ c , c' ]) (r : ⟨ R ⟅ c' , d ⟆b ⟩)
              → PH-ob ((R ⟪ f ⟫l) r) ≡ (S ⟪ f ⟫l) (PH-ob r)
      PH-natR : ∀ {c d d'} (r : ⟨ R ⟅ c , d ⟆b ⟩) (g : D [ d , d' ])
              → PH-ob ((R ⟪ g ⟫r) r) ≡ (S ⟪ g ⟫r) (PH-ob r)

  open ProfHomo

  -- A definition of profunctor homomorphism without implicit arguments
  -- so that it'll work with the reflection library
  record ProfHomo' : Type ℓmaxCDSR where
    field
      PH-ob : ∀ c d → (r : ⟨ R ⟅ c , d ⟆b ⟩) → ⟨ S ⟅ c , d ⟆b ⟩
      PH-natL : ∀ c c' d (f : C [ c , c' ]) (r : ⟨ R ⟅ c' , d ⟆b ⟩)
              → PH-ob c d ((R ⟪ f ⟫l) r) ≡ (S ⟪ f ⟫l) (PH-ob c' d r)
      PH-natR : ∀ c d d' (r : ⟨ R ⟅ c , d ⟆b ⟩) (g : D [ d , d' ])
              → PH-ob c d' ((R ⟪ g ⟫r) r) ≡ (S ⟪ g ⟫r) (PH-ob c d r)

  isProp-natL : (PH' : ProfHomo') →
              isProp (∀ c c' d (f : C [ c , c' ]) (r : ⟨ R ⟅ c' , d ⟆b ⟩)
              → ProfHomo'.PH-ob PH' c d ((R ⟪ f ⟫l) r) ≡
                (S ⟪ f ⟫l) (ProfHomo'.PH-ob PH' c' d r))
  isProp-natL PH' =
    isPropΠ5
    (λ x y z w v →
      str (S ⟅ x , z ⟆b)
        (ProfHomo'.PH-ob PH' x z ((R ⟪ w ⟫l) v))
        ((S ⟪ w ⟫l) (ProfHomo'.PH-ob PH' y z v))
    )

  isProp-natR : (PH' : ProfHomo') →
                isProp (∀ c d d' (r : ⟨ R ⟅ c , d ⟆b ⟩) (g : D [ d , d' ])
              → ProfHomo'.PH-ob PH' c d' ((R ⟪ g ⟫r) r) ≡
                (S ⟪ g ⟫r) (ProfHomo'.PH-ob PH' c d r))
  isProp-natR PH' =
    isPropΠ5
    (λ x y z w v →
      str (S ⟅ x , z ⟆b)
        (ProfHomo'.PH-ob PH' x z ((R ⟪ v ⟫r) w))
        ((S ⟪ v ⟫r) (ProfHomo'.PH-ob PH' x y w))
    )

  -- Use reflection to reason about equivalence of ProfHomo' and an
  -- iterated Σ type
  -- We can then use this Σ type to define paths between instances of ProfHomo'
  unquoteDecl ProfHomo'IsoΣ =
    declareRecordIsoΣ ProfHomo'IsoΣ (quote (ProfHomo'))

  -- The explicit and implicit versions of ProfHomo are indeed the same
  isoProfHomoProfHomo' : Iso ProfHomo ProfHomo'
  isoProfHomoProfHomo' =
    iso
    (λ x → record {
      PH-ob = λ c d r → x .PH-ob {c = c} {d = d} r ;
      PH-natL = λ c c' d f r → x .PH-natL {c = c} {c' = c'} {d = d} f r ;
      PH-natR = λ c d d' r g → x .PH-natR {c = c} {d = d} {d' = d'} r g
    })
    (λ x → record {
      PH-ob = λ {c} {d} r → ProfHomo'.PH-ob x c d r ;
      PH-natL = λ {c}{c'}{d} f r → ProfHomo'.PH-natL x c c' d f r ;
      PH-natR = λ {c}{d}{d'} r g → ProfHomo'.PH-natR x c d d' r g
    })
    (λ _ → refl)
    (λ _ → refl)

  ProfIso : Type _
  ProfIso = Σ[ ϕ ∈ ProfHomo ] ∀ c d → isIso (ϕ .PH-ob {c}{d})

open ProfHomo
module _  {C : Category ℓC ℓC'}{D : Category ℓD ℓD'} {ℓS : Level} where
  -- Product of a presheaf with a profunctor
  -- This could be done by turning the presheaf into a profunctor
  -- first but at the cost of extra ids.
  _o×_ : (P : 𝓟o C ℓS) → (R : C o-[ ℓS ]-* D) → C o-[ ℓS ]-* D
  (P o× R) = mkBifunctorParAx F where
    open BifunctorParAx
    F : BifunctorParAx (C ^op) D (SET ℓS)
    F .Bif-ob c d = (⟨ P ⟅ c ⟆ ⟩ × ⟨  R ⟅ c , d ⟆b ⟩)
      , (isSet× ((P ⟅ c ⟆) .snd) ((R ⟅ c , d ⟆b) .snd))
    F .Bif-homL f _ (p , r) = (P ⟪ f ⟫) p , (R ⟪ f ⟫l) r
    F .Bif-homR _ g (p , r) = p , ((R ⟪ g ⟫r) r)
    F .Bif-hom× f g (p , r) = ((P ⟪ f ⟫) p) , ((R ⟪ f , g ⟫×) r)
    F .Bif-×-id = funExt (λ (p , r) → ΣPathP ((funExt⁻ (P .F-id) _)
      , funExt⁻ (R .Bif-×-id) _))
    F .Bif-×-seq f f' g g' = funExt (λ (p , r) → ΣPathP (
      ( funExt⁻ (P .F-seq f f') _)
      , funExt⁻ (R .Bif-×-seq f f' g g') _))
    F .Bif-L×-agree f = funExt (λ (p , r) → ΣPathP (refl
      , (funExt⁻ (R .Bif-L×-agree _) _)))
    F .Bif-R×-agree g = funExt (λ (p , r) → ΣPathP ((sym (funExt⁻ (P .F-id) _))
      , funExt⁻ (R .Bif-R×-agree _) _))

Functor→Prof*-o : (C : Category ℓC ℓC')
                  (D : Category ℓD ℓD') (F : Functor C D) → C *-[ ℓD' ]-o D
Functor→Prof*-o C D F = HomBif D ∘Fr F

Functor→Profo-* : (C : Category ℓC ℓC')
                  (D : Category ℓD ℓD') (F : Functor C D) → C o-[ ℓD' ]-* D
Functor→Profo-* C D F = HomBif D ∘Fl (F ^opF)

-- Prof*-o→Functor : (C : Category ℓC ℓC')
--                   (D : Category ℓD ℓD') (R : C *-[ ℓS ]-o D) →
--                     Functor C (FUNCTOR (D ^op) (SET ℓS))
-- Prof*-o→Functor C D R = curryFl (D ^op) (SET _) ⟅ Bifunctor→Functor R ⟆

-- Profo-*→Functor : (C : Category ℓC ℓC')
--                   (D : Category ℓD ℓD') (R : C o-[ ℓS ]-* D) →
--                     Functor (C ^op) (FUNCTOR D (SET ℓS))
-- Profo-*→Functor C D R = curryF D (SET _) ⟅ Bifunctor→Functor R ⟆

module _ (C : Category ℓC ℓC') (D : Category ℓD ℓD') (R : C *-[ ℓS ]-o D) where

  open NatTrans
  open NatIso
  open isIsoC
  open isEquiv

  UniversalElementAt : C .ob → Type _
  UniversalElementAt c = UniversalElement D (appR R c)

  UniversalElements : Type _
  UniversalElements = ((∀ (c : C .ob) → UniversalElement D (appR R c)))

  FunctorComprehension :
    ((∀ (c : C .ob) → UniversalElement D (appR R c)))
    → Σ[ F ∈ Functor C D ] (∀ (c : C .ob)
    → UniversalElementOn D (appR R c) (F ⟅ c ⟆))
  FunctorComprehension ues = F ,
    (λ c → UniversalElementToUniversalElementOn _ _ (ues c)) where
    F : Functor C D
    F .F-ob c = ues c .vertex
    F .F-hom f =
      ues _ .universal _ .equiv-proof ((R ⟪ f ⟫r) (ues _ .element))
      .fst .fst
    F .F-id {x = c} = cong fst (ues c .universal (ues c .vertex) .equiv-proof
      ((R ⟪ C .id ⟫r) (ues _ .element)) .snd (_ ,
      funExt⁻ (R .Bif-L-id) _
      ∙ sym (funExt⁻ (R .Bif-R-id) _)))
    F .F-seq f g = cong fst ((ues _ .universal (ues _ .vertex) .equiv-proof
      ((R ⟪ f ⋆⟨ C ⟩ g ⟫r) (ues _ .element))) .snd (_ ,
      funExt⁻ (R .Bif-L-seq _ _) _
      ∙ cong (R .Bif-homL _ _) (ues _ .universal _ .equiv-proof
          ((R ⟪ g ⟫r) (ues _ .element)) .fst .snd)
      ∙ funExt⁻ ( (Bif-RL-commute R _ _)) _
      ∙ cong (R .Bif-homR _ _) ((ues _ .universal _ .equiv-proof
          ((R ⟪ f ⟫r) (ues _ .element)) .fst .snd))
      ∙ sym (funExt⁻ (R .Bif-R-seq _ _) _) ))

  UniqueFunctorComprehension :
    isUnivalent D
    → (∀ (c : C .ob) → UniversalElement D (appR R c))
    → ∃![ F ∈ Functor C D ] (∀ (c : C .ob)
    → UniversalElementOn D (appR R c) (F ⟅ c ⟆))
  UniqueFunctorComprehension isUnivD ues =
    (F , universalAtF) ,
    (λ (G , universalAtG) →
      ΣPathP (
        the-functor-path G universalAtG isUnivD ,
        funExt (λ c → {!universalAtG c .fst!})
      )
    )
    where
    F : Functor C D
    F = FunctorComprehension ues .fst

    universalAtF : _
    universalAtF = FunctorComprehension ues .snd

    the-functor-path : (G : Functor C D)
      → (∀ (c : C .ob) → UniversalElementOn D (appR R c) (G ⟅ c ⟆))
      → isUnivalent D
      → F ≡ G
    the-functor-path G universalAtG isUnivD = {!universalAtG!}

    the-ue-path : {G : Functor C D} → isUnivalent D → F ≡ G
      → (universalAtG : ∀ (c : C .ob) → UniversalElementOn D (appR R c) (G ⟅ c ⟆))
      → (∀ (c : C .ob)
        → PathP (λ i → (appR R c ⟅ (the-functor-path G universalAtG isUnivD (~ i)) ⟅ c ⟆ ⟆) .fst)
          (universalAtG c .fst) (universalAtF c .fst))
    the-ue-path {G} isUnivD p universalAtG c = ?


  -- ProfRepresents : Functor C D → Type _
  -- ProfRepresents G = ProfIso {C = D}{D = C} R (Functor→Prof*-o C D G)

  -- ProfRepresentation : Type _
  -- ProfRepresentation = Σ[ G ∈ Functor C D ] ProfRepresents G

  -- PshFunctorRepresentation : Type _
  -- PshFunctorRepresentation =
  --   Σ[ G ∈ Functor C D ]
  --   NatIso (Prof*-o→Functor C D ((LiftF {ℓS}{ℓD'}) ∘Fb R ))
  --          (Prof*-o→Functor C D (LiftF {ℓD'}{ℓS} ∘Fb (Functor→Prof*-o C D G)))

  -- RepresentableAt : (c : C .ob) → Type _
  -- RepresentableAt c = UniversalElement D (pAppR R c)

  -- ParamUnivElt : Type _
  -- ParamUnivElt = (c : C .ob) → RepresentableAt c

  -- ParamUniversalElement : Type _
  -- ParamUniversalElement = (c : C .ob) → UniversalElement D (pAppR R c)

  -- {-
  --   ProfRepresentation, PshFunctorRepresentation, ParamUnivElt,
  --     and ParamUniversalElement
  --   each give a different criterion for a profunctor R to be representable.

  --   These are all equivalent, and the equivalence is witnessed by
  --     the following functions.
  --   Below we simply provide the functions, and in Profunctor.Equivalence
  --     we prove
  --   that they do indeed provide type isomorphisms.
  -- -}

  -- -- ProfRepresentation → PshFunctorRepresentation
  -- ProfRepresentation→PshFunctorRepresentation : ProfRepresentation →
  --                                               PshFunctorRepresentation
  -- ProfRepresentation→PshFunctorRepresentation (G , η) =
  --   G ,
  --   record {
  --     trans = the-trans ;
  --     nIso = λ c →
  --       FUNCTORIso
  --         (D ^op)
  --         (SET (ℓ-max ℓD' ℓS))
  --         (the-trans .N-ob c)
  --         λ d →
  --           isiso
  --             (λ x → lift ((η .snd d c .fst) (lower x)))
  --             (λ i x → lift ((η .snd d c .snd .fst) (lower x) i))
  --             (λ i x → lift ((η .snd d c .snd .snd) (lower x) i))
  --     }
  --     where
  --     the-trans : NatTrans (Prof*-o→Functor C D (bifCompF LiftF R))
  --       (Prof*-o→Functor C D (bifCompF LiftF (Functor→Prof*-o C D G)))
  --     the-trans .N-ob c =
  --       natTrans
  --         (λ d x → lift (η .fst .PH-ob (lower x)))
  --         (λ f → funExt (λ x →
  --           (Prof*-o→Functor C D (bifCompF LiftF R) .F-ob c .F-hom f
  --             ⋆f
  --             (λ x₂ → lift (η .fst .PH-ob (lower x₂)))) x
  --             ≡⟨ (λ i → lift (η .fst .PH-ob (((R ⟪ f ⟫l) ⋆f
  --               R .Bif-idR i) (lower x)))) ⟩
  --           lift (PH-ob (η .fst) ((R ⟪ f ⟫l) (lower x)))
  --             ≡⟨ (λ i → lift (η .fst .PH-natL f (lower x) i)) ⟩
  --           lift ((Functor→Prof*-o C D G ⟪ f ⟫l) (PH-ob (η .fst) (lower x)))
  --             ≡⟨ (λ i → lift (((Functor→Prof*-o C D G) ⟪ f ⟫l ⋆f
  --               Functor→Prof*-o C D G .Bif-idR (~ i))
  --                 (η .fst .PH-ob (lower x)))) ⟩
  --           ((λ x₂ → lift (η .fst .PH-ob (lower x₂)))
  --             ⋆f
  --             Prof*-o→Functor C D (bifCompF LiftF (Functor→Prof*-o C D G))
  --               .F-ob c .F-hom f) x ∎
  --            ))
  --     the-trans .N-hom f =
  --       makeNatTransPath
  --             (funExt (λ d → funExt λ x →
  --               lift (η .fst .PH-ob ((Bif-homL R (id D) _ ⋆f
  --                 (R ⟪ f ⟫r)) (lower x)))
  --                 ≡⟨ (λ i → lift (η .fst .PH-ob ((R .Bif-idL i ⋆f
  --                   (R ⟪ f ⟫r)) (lower x)))) ⟩
  --               lift (PH-ob (η .fst) ((R ⟪ f ⟫r) (lower x)))
  --                 ≡⟨ (λ i → lift (η .fst .PH-natR (lower x) f i)) ⟩
  --               lift ((Functor→Prof*-o C D G ⟪ f ⟫r) (PH-ob (η .fst) (lower x)))
  --                 ≡⟨ ((λ i → lift ((Functor→Prof*-o C D G .Bif-idL (~ i) ⋆f
  --                   (Functor→Prof*-o C D G ⟪ f ⟫r ))
  --                     (η .fst .PH-ob (lower x))))) ⟩
  --               lift
  --                 ((Bif-homL (Functor→Prof*-o C D G) (id D) _ ⋆f
  --                   (Functor→Prof*-o C D G ⟪ f ⟫r))
  --                  (η .fst .PH-ob (lower x))) ∎))

  -- -- PshFunctor Representation → ProfRepresentation
  -- PshFunctorRepresentation→ProfRepresentation : PshFunctorRepresentation →
  --                                               ProfRepresentation
  -- PshFunctorRepresentation→ProfRepresentation (G , η) =
  --   G ,
  --   (record {
  --     PH-ob = λ {d}{c} r → lower ((η .trans .N-ob c .N-ob d) (lift r)) ;
  --     PH-natL = λ {d}{d'}{c} f r →
  --       lower (((η .trans .N-ob c .N-ob d) ∘f
  --         ((bifCompF LiftF R) .Bif-homL f c)) (lift r))
  --        ≡⟨ ((λ i → lower (((η .trans .N-ob c .N-ob d) ∘f
  --          ( (bifCompF LiftF R) .Bif-homL f c ⋆f
  --            (bifCompF LiftF R) .Bif-idR (~ i))) (lift r)))) ⟩
  --       lower (((η .trans .N-ob c .N-ob d) ∘f
  --         (((bifCompF LiftF R) .Bif-homL f c) ⋆f
  --           (bifCompF LiftF R) .Bif-homR d (C .id))) (lift r))
  --        ≡⟨ ((λ i → lower ((η .trans .N-ob c .N-hom f i) (lift r)))) ⟩
  --       lower ((N-ob (η .trans .N-ob c) d' ⋆f
  --         Prof*-o→Functor C D (bifCompF LiftF (Functor→Prof*-o C D G))
  --           .F-ob c .F-hom f) (lift r))
  --        ≡⟨ ((λ i → ((Functor→Prof*-o C D G ⟪ f ⟫l) ⋆f
  --          (Functor→Prof*-o C D G) .Bif-idR i)
  --            (lower (η .trans .N-ob c .N-ob d' (lift r))))) ⟩
  --       (Functor→Prof*-o C D G ⟪ f ⟫l)
  --         (lower (η .trans .N-ob c .N-ob d' (lift r))) ∎
  --      ;
  --     PH-natR = λ {c}{d}{d'} r g →
  --       lower (η .trans .N-ob d' .N-ob c (lift ((R ⟪ g ⟫r) r)))
  --         ≡⟨ (λ i → lower (η .trans .N-ob d' .N-ob c
  --           (lift ((R .Bif-idL (~ i) ⋆f R ⟪ g ⟫r) r)))) ⟩
  --       lower
  --         ((Prof*-o→Functor C D (bifCompF LiftF R) .F-hom g .N-ob c ⋆f
  --           N-ob (η .trans) d' .N-ob c) (lift r))
  --         ≡⟨ (λ i → lower ((η .trans .N-hom g i .N-ob c) (lift r))) ⟩
  --       lower ((N-ob (η .trans) d .N-ob c ⋆f
  --         Prof*-o→Functor C D (bifCompF LiftF (Functor→Prof*-o C D G))
  --           .F-hom g .N-ob c) (lift r))
  --         ≡⟨ ((λ i → (Functor→Prof*-o C D G .Bif-idL i ⋆f
  --           (Functor→Prof*-o C D G ⟪ g ⟫r))
  --             (lower (η .trans .N-ob d .N-ob c (lift r))))) ⟩
  --       (Functor→Prof*-o C D G ⟪ g ⟫r)
  --         (lower (η .trans .N-ob d .N-ob c (lift r))) ∎
  --     }) ,
  --   λ d c →
  --     (λ x → lower (η .nIso c .inv .N-ob d (lift x))) ,
  --     (λ x i → lower ((η .nIso c .sec i .N-ob d) (lift x))) ,
  --     (λ x i → lower((η .nIso c .ret i .N-ob d) (lift x)))

  -- open NatIso
  -- open NatTrans
  -- open isIsoC

  -- -- -- PshFunctorRepresentation → ParamUnivElt
  -- -- PshFunctorRepresentation→ParamUnivElt : PshFunctorRepresentation →
  -- --                                         ParamUnivElt
  -- -- PshFunctorRepresentation→ParamUnivElt (G , η) = (λ c →
  -- --   let R⟅-,c⟆ = (pAppR R c) in
  -- --   let η⁻¹ = symNatIso η in
  -- --     record {
  -- --       vertex = (G ⟅ c ⟆) ;
  -- --       element = lower ((η⁻¹ .trans .N-ob c .N-ob (G ⟅ c ⟆)) (lift (D .id))) ;
  -- --       universal = record {
  -- --         coinduction = λ {d} ϕ → lower ((η .trans .N-ob c .N-ob d) (lift ϕ));
  -- --         commutes = (λ {d} ϕ →
  -- --           let coindϕ = (lower ((η .trans .N-ob c .N-ob d) (lift ϕ))) in
  -- --           lower (((LiftF ∘F R⟅-,c⟆) ⟪ coindϕ ⟫)
  -- --             ((η⁻¹ .trans .N-ob c .N-ob (G ⟅ c ⟆)) (lift (D .id))))
  -- --             ≡⟨ (λ i → lower (((LiftF ∘Fb R ) .Bif-idR (~ i))
  -- --               (((LiftF ∘Fb R ) .Bif-homL coindϕ c)
  -- --                 ((η⁻¹ .trans .N-ob c .N-ob (G ⟅ c ⟆)) (lift (D .id)))))) ⟩
  -- --           lower ((((Prof*-o→Functor C D ((LiftF {ℓS}{ℓD'}) ∘Fb R )) ⟅ c ⟆)
  -- --           ⟪ coindϕ ⟫) ((η⁻¹ .trans .N-ob c .N-ob (G ⟅ c ⟆)) (lift (D .id))))
  -- --             ≡⟨ (λ i → lower ((((η⁻¹ .trans .N-ob c .N-hom coindϕ) (~ i))
  -- --               (lift (D .id))))) ⟩
  -- --           lower ((η⁻¹ .trans .N-ob c .N-ob d)
  -- --             (((Bifunctor→Functor ((LiftF {ℓD'}{ℓS}) ∘Fb (HomBif D)))
  -- --               ⟪ coindϕ , G ⟪ C .id ⟫ ⟫) (lift (D .id))))
  -- --             ≡⟨ ( λ i → lower ((η⁻¹ .trans .N-ob c .N-ob d)
  -- --             (((Bifunctor→Functor ((LiftF {ℓD'}{ℓS}) ∘Fb (HomBif D)))
  -- --               ⟪ coindϕ , G .F-id (i) ⟫) (lift (D .id))))) ⟩
  -- --           lower ((η⁻¹ .trans .N-ob c .N-ob d)
  -- --             (((Bifunctor→Functor ((LiftF {ℓD'}{ℓS}) ∘Fb (HomBif D)))
  -- --               ⟪ coindϕ , D .id ⟫) (lift (D .id))))
  -- --             ≡⟨ (λ i →
  -- --               lower ((η⁻¹ .trans .N-ob c .N-ob d)
  -- --                 ((((LiftF {ℓD'}{ℓS}) ∘Fb (HomBif D)) .Bif-idR (i))
  -- --                 ((((LiftF {ℓD'}{ℓS}) ∘Fb (HomBif D)) .Bif-homL coindϕ
  -- --                   (G ⟅ c ⟆)) (lift (D .id))))
  -- --               )
  -- --               ) ⟩
  -- --           lower ((η⁻¹ .trans .N-ob c .N-ob d) (lift (coindϕ ⋆⟨ D ⟩ (D .id))))
  -- --             ≡⟨ (λ i → lower ((η⁻¹ .trans .N-ob c .N-ob d)
  -- --               (lift (D .⋆IdR coindϕ (i))))) ⟩
  -- --           lower ((η⁻¹ .trans .N-ob c .N-ob d) (lift (coindϕ)))
  -- --             ≡⟨ (λ i → lower ((((η .nIso c .ret) (i)) .N-ob d) (lift ϕ))) ⟩
  -- --           ϕ ∎) ;
  -- --         is-uniq =
  -- --           λ {d} ϕ f ε⋆f≡ϕ →
  -- --           let coindϕ = (lower ((η .trans .N-ob c .N-ob d) (lift ϕ))) in
  -- --             f
  -- --               ≡⟨ sym (D .⋆IdR f) ⟩
  -- --             (f ⋆⟨ D ⟩ D .id)
  -- --               ≡⟨ (λ i → (((HomBif D) .Bif-idR (~ i))
  -- --                 (((HomBif D) .Bif-homL f (G ⟅ c ⟆)) (D .id)))) ⟩
  -- --             (((Bifunctor→Functor (HomBif D)) ⟪ f , D .id ⟫) (D .id))
  -- --               ≡⟨ (λ i → (((Bifunctor→Functor (HomBif D))
  -- --                 ⟪ f , G .F-id (~ i) ⟫) (D .id))) ⟩
  -- --             (((Bifunctor→Functor (HomBif D)) ⟪ f , G ⟪ C .id ⟫ ⟫) (D .id))
  -- --               ≡⟨ (λ i → lower(((η .nIso c .sec) (~ i) .N-ob d)
  -- --                 (lift (((Bifunctor→Functor (HomBif D))
  -- --                   ⟪ f , G ⟪ C .id ⟫ ⟫) (D .id))))) ⟩
  -- --             lower ((η .trans .N-ob c .N-ob d)
  -- --               ((η⁻¹ .trans .N-ob c .N-ob d)
  -- --               (lift (((Bifunctor→Functor (HomBif D))
  -- --                 ⟪ f , G ⟪ C .id ⟫ ⟫) (D .id)))))
  -- --               ≡⟨ (λ i → lower ((η .trans .N-ob c .N-ob d)
  -- --                 (((η⁻¹ .trans .N-ob c .N-hom f) (i)) (lift (D .id))))) ⟩
  -- --             lower ((η .trans .N-ob c .N-ob d)
  -- --             ((((Prof*-o→Functor C D ((LiftF {ℓS}{ℓD'}) ∘Fb R )) ⟅ c ⟆) ⟪ f ⟫)
  -- --               ((η⁻¹ .trans .N-ob c .N-ob (G ⟅ c ⟆)) (lift (D .id)))))
  -- --               ≡⟨ ( λ i → lower ((η .trans .N-ob c .N-ob d)
  -- --               (((LiftF ∘Fb R ) .Bif-idR (i)) (((LiftF ∘Fb R ) .Bif-homL f c)
  -- --               ((η⁻¹ .trans .N-ob c .N-ob (G ⟅ c ⟆)) (lift (D .id))))))) ⟩
  -- --             lower ((η .trans .N-ob c .N-ob d) (lift ((R⟅-,c⟆ ⟪ f ⟫)
  -- --             (lower ((η⁻¹ .trans .N-ob c .N-ob (G ⟅ c ⟆)) (lift (D .id)))))))
  -- --               ≡⟨ (λ i →  (lower ((η .trans .N-ob c .N-ob d)
  -- --                 (lift (ε⋆f≡ϕ i))))) ⟩
  -- --             coindϕ ∎
  -- --       }
  -- --     }
  -- --   )

  -- -- ParamUnivElt→Functor : ParamUnivElt → Functor C D
  -- -- ParamUnivElt→Functor ues .F-ob c = ues c .vertex
  -- -- ParamUnivElt→Functor ues .F-hom {x = c}{y = c'} f =
  -- --   ues c' .universal .coinduction ((R ⟪ f ⟫r) (ues c .element))
  -- -- ParamUnivElt→Functor ues .F-id {x = c} =
  -- --   cong (ues c .universal .coinduction) (λ i → R .Bif-idR i (ues c .element))
  -- --   ∙ sym (coinduction-elt (ues c .universal))
  -- -- ParamUnivElt→Functor ues .F-seq {x = c}{y = c'}{z = c''} f g =
  -- --   -- Both sides are ≡ to R .Bif-homR (ues c .vertex) g
  -- --     -- (R .Bif-homR (ues c .vertex) f (ues c .element))
  -- --   cong (ues c'' .universal .coinduction)
  -- --   ((λ i → R .Bif-seqR f g i (ues c .element)))
  -- --   ∙ cong (coinduction (ues c'' .universal))
  -- --       ( cong (R .Bif-homR (ues c .vertex) g)
  -- --         (sym (ues c' .universal .commutes _))
  -- --       ∙ (λ i → R .Bif-assoc (ues c' .universal .coinduction ((R ⟪ f ⟫r)
  -- --         (ues c .element))) g i (ues c' .element)))
  -- --   ∙ sym (coinduction-natural (ues c'' .universal) _ _)

  -- -- -- ParamUnivElt → PshFunctorRepresentation
  -- -- ParamUnivElt→PshFunctorRepresentation : ParamUnivElt →
  -- --                                         PshFunctorRepresentation
  -- -- ParamUnivElt→PshFunctorRepresentation ues =
  -- --   (representing-functor , representing-nat-iso) where
  -- --   representing-functor : Functor C D
  -- --   representing-functor = ParamUnivElt→Functor ues

  -- --   rep-nat-iso-trans : (c : C .ob) →
  -- --     NatTrans (Prof*-o→Functor C D (LiftF {ℓS}{ℓD'} ∘Fb R) .F-ob c)
  -- --              (Prof*-o→Functor C D (LiftF {ℓD'}{ℓS} ∘Fb
  -- --                (Functor→Prof*-o C D representing-functor)) .F-ob c)
  -- --   rep-nat-iso-trans c .N-ob d  =
  -- --     let R⟅-,c⟆ = (pAppR R c) in
  -- --     (λ f → lift {ℓD'}{ℓS} ((ues c) .universal .coinduction {b = d}
  -- --       (lower {ℓS}{ℓD'} f)))
  -- --   rep-nat-iso-trans c .N-hom {d}{d'} ϕ =
  -- --     let R⟅-,c⟆ = (pAppR R c) in
  -- --     let εc = ues c .element in
  -- --     let coind = (ues c) .universal .coinduction in
  -- --     funExt λ x →
  -- --       lift (coind (((Prof*-o→Functor C D R .F-ob c) ⟪ ϕ ⟫) (lower x)))
  -- --         ≡⟨ ( λ i → lift (coind ((R .Bif-idR (i)) ((R .Bif-homL ϕ c)
  -- --           (lower x))))) ⟩
  -- --       lift (coind (D [ (lower x) ∘ᴾ⟨ R⟅-,c⟆ ⟩ ϕ ] ))
  -- --         ≡⟨ (λ i → lift ((coinduction-natural ((ues c) .universal)
  -- --           (lower x) ϕ) (~ i))) ⟩
  -- --       lift ((coind (lower x)) ∘⟨ D ⟩ ϕ )
  -- --         ≡⟨ (λ i → lift (((HomBif D) .Bif-idR (~ i))
  -- --           (((HomBif D) .Bif-homL ϕ _) (coind (lower x)))) ) ⟩
  -- --       lift (((Bifunctor→Functor (HomBif D)) ⟪ ϕ , D .id ⟫ ) (coind (lower x)))
  -- --         ≡⟨ (λ i → lift (((Bifunctor→Functor (HomBif D))
  -- --           ⟪ ϕ , representing-functor .F-id (~ i) ⟫ ) (coind (lower x)))) ⟩
  -- --       lift (((Bifunctor→Functor (HomBif D))
  -- --         ⟪ ϕ , representing-functor ⟪ C . id ⟫ ⟫ ) (coind (lower x))) ∎

  -- --   representing-nat-iso  : NatIso
  -- --       (Prof*-o→Functor C D (LiftF {ℓS}{ℓD'} ∘Fb R))
  -- --       (Prof*-o→Functor C D (LiftF {ℓD'}{ℓS} ∘Fb
  -- --         (Functor→Prof*-o C D representing-functor)))
  -- --   representing-nat-iso .trans .N-ob c = rep-nat-iso-trans c
  -- --   representing-nat-iso .trans .N-hom {x}{y} ψ =
  -- --     let R⟅-,x⟆ = (pAppR R x) in
  -- --     let R⟅-,y⟆ = (pAppR R y) in
  -- --     let εy = ues y .element in
  -- --     let εx = ues x .element in
  -- --     let coindx = ues x .universal .coinduction in
  -- --     let coindy = ues y .universal .coinduction in
  -- --     makeNatTransPath (funExt (λ d → funExt (λ α →
  -- --         lift (coindy (((Bifunctor→Functor R) ⟪ D .id , ψ ⟫) (lower α)))
  -- --           ≡⟨ (λ i → lift (coindy
  -- --             (R .Bif-homR _ ψ ((R .Bif-idL (i)) (lower α))))) ⟩
  -- --         lift (coindy (R .Bif-homR _ ψ (lower α)))
  -- --           ≡⟨ ( λ i → lift (ues y .universal .is-uniq
  -- --                 (R .Bif-homR _ ψ (lower α))
  -- --                 ((coindx (lower α)) ⋆⟨ D ⟩ (representing-functor ⟪ ψ ⟫))
  -- --                 (
  -- --                 (
  -- --                   D [ εy ∘ᴾ⟨ R⟅-,y⟆ ⟩ (coindy ((R .Bif-homR _ ψ) εx) ∘⟨ D ⟩
  -- --                     (coindx (lower α))) ]
  -- --                     ≡⟨ (λ i → D [
  -- --                       εy ∘ᴾ⟨ R⟅-,y⟆ ⟩ ((coinduction-natural (ues y .universal)
  -- --                       ((R .Bif-homR _ ψ) εx) (coindx (lower α))) i)]  ) ⟩
  -- --                   D [ εy ∘ᴾ⟨ R⟅-,y⟆ ⟩
  -- --                     coindy ( D [ ((R .Bif-homR _ ψ) εx) ∘ᴾ⟨ R⟅-,y⟆ ⟩
  -- --                       (coindx (lower α)) ]) ]
  -- --                     ≡⟨ ues y .universal .commutes
  -- --                       (D [ ((R .Bif-homR _ ψ) εx) ∘ᴾ⟨ R⟅-,y⟆ ⟩
  -- --                         (coindx (lower α)) ]) ⟩
  -- --                   D [ ((R .Bif-homR _ ψ) εx) ∘ᴾ⟨ R⟅-,y⟆ ⟩ (coindx (lower α)) ]
  -- --                    ≡⟨ (λ i → ((R .Bif-assoc (coindx (lower α)) ψ) (~ i)) εx) ⟩
  -- --                   (R .Bif-homR _ ψ) (D [ εx ∘ᴾ⟨ R⟅-,x⟆ ⟩ (coindx (lower α)) ])
  -- --                    ≡⟨ (λ i → (R .Bif-homR _ ψ)
  -- --                      (ues x .universal .commutes (lower α) (i))) ⟩
  -- --                   (R .Bif-homR _ ψ (lower α)) ∎
  -- --                 )
  -- --                 )
  -- --                 (~ i))) ⟩
  -- --         lift ((coindx (lower α)) ⋆⟨ D ⟩ (representing-functor ⟪ ψ ⟫))
  -- --           ≡⟨ (λ i → lift ((HomBif D) .Bif-homR _ (representing-functor ⟪ ψ ⟫)
  -- --             (((HomBif D) .Bif-idL (~ i)) (coindx (lower α))))) ⟩
  -- --         lift (((Bifunctor→Functor (HomBif D)) ⟪ D .id ,
  -- --           representing-functor ⟪ ψ ⟫ ⟫) (coindx (lower α))) ∎

  -- --     )))
  -- --   representing-nat-iso .nIso c .inv .N-ob d =
  -- --     let εc = ues c .element in
  -- --     let R⟅-,c⟆ = (pAppR R c) in
  -- --     λ f → lift (D [ εc ∘ᴾ⟨ R⟅-,c⟆ ⟩ (lower f) ])
  -- --   representing-nat-iso .nIso c .inv .N-hom {d}{d'} ϕ =
  -- --     let εc = ues c .element in
  -- --     let R⟅-,c⟆ =(pAppR R c) in
  -- --     funExt λ x →
  -- --       lift (D [ εc ∘ᴾ⟨ R⟅-,c⟆ ⟩ ((Bifunctor→Functor (HomBif D))
  -- --         ⟪ ϕ , representing-functor ⟪ C .id ⟫ ⟫) (lower x) ])
  -- --         ≡⟨ (λ i → lift (D [ εc ∘ᴾ⟨ R⟅-,c⟆ ⟩ ((Bifunctor→Functor (HomBif D))
  -- --           ⟪ ϕ , representing-functor .F-id i ⟫) (lower x) ])) ⟩
  -- --       lift (D [ εc ∘ᴾ⟨ R⟅-,c⟆ ⟩ ((Bifunctor→Functor (HomBif D))
  -- --         ⟪ ϕ , D .id ⟫ ) (lower x) ])
  -- --         ≡⟨ (λ i → lift (D [ εc ∘ᴾ⟨ R⟅-,c⟆ ⟩ ((HomBif D) .Bif-idR (i)
  -- --           (((HomBif D) .Bif-homL ϕ _) (lower x))) ])) ⟩
  -- --       lift (D [ εc ∘ᴾ⟨ R⟅-,c⟆ ⟩ (ϕ ⋆⟨ D ⟩ (lower x)) ])
  -- --         ≡⟨ (λ i → lift (((R⟅-,c⟆ .F-seq (lower x) ϕ) i) εc)) ⟩
  -- --       lift ((R .Bif-homL ϕ _) (D [ εc ∘ᴾ⟨ R⟅-,c⟆ ⟩ (lower x) ]))
  -- --         ≡⟨ (λ i → lift ((R .Bif-idR (~ i)) ((R .Bif-homL ϕ _)
  -- --           (D [ εc ∘ᴾ⟨ R⟅-,c⟆ ⟩ (lower x) ])))) ⟩
  -- --       lift (((Bifunctor→Functor R) ⟪ ϕ , C .id ⟫)
  -- --         (D [ εc ∘ᴾ⟨ R⟅-,c⟆ ⟩ (lower x) ])) ∎

  -- --   representing-nat-iso .nIso c .sec =
  -- --     let R⟅-,c⟆ = (pAppR R c) in
  -- --     makeNatTransPath (funExt λ d → funExt λ x → (λ i →
  -- --       lift ((η-expansion ((ues c) .universal) (lower x)) (~ i))) )
  -- --   representing-nat-iso .nIso c .ret =
  -- --     let R⟅-,c⟆ = (pAppR R c) in
  -- --     makeNatTransPath (funExt λ d → funExt λ x → (λ i →
  -- --       lift (((ues c) .universal .commutes (lower x)) i)))

  -- -- -- ParamUniversalElement → ParamUnivElt
  -- -- ParamUniversalElement→ParamUnivElt : ParamUniversalElement → ParamUnivElt
  -- -- ParamUniversalElement→ParamUnivElt U c =
  -- --   UniversalElement→UnivElt D (pAppR R c) (U c)

  -- -- -- ParamUnivElt → ParamUniversalElement
  -- -- ParamUnivElt→ParamUniversalElement : ParamUnivElt → ParamUniversalElement
  -- -- ParamUnivElt→ParamUniversalElement U c =
  -- --   UnivElt→UniversalElement D (pAppR R c) (U c)

  -- -- {-
  -- --   We have now given maps
  -- --     ProfRepresentation ⇔ PshFunctorRepresentation
  -- --     PshFunctorRepresentation ⇔ ParamUnivElt
  -- --     ParamUnivElt ⇔ ParamUniversalElement

  -- --   For convenience,
  -- --   below we also stitch these together to give all pairwise maps.
  -- -- -}

  -- -- -- ProfRepresentation → ParamUnivElt
  -- -- ProfRepresentation→ParamUnivElt : ProfRepresentation → ParamUnivElt
  -- -- ProfRepresentation→ParamUnivElt R =
  -- --   PshFunctorRepresentation→ParamUnivElt
  -- --     (ProfRepresentation→PshFunctorRepresentation R)

  -- -- -- ProfRepresentation → ParamUniversalElement
  -- -- ProfRepresentation→ParamUniversalElement : ProfRepresentation →
  -- --                                            ParamUniversalElement
  -- -- ProfRepresentation→ParamUniversalElement R =
  -- --   ParamUnivElt→ParamUniversalElement (ProfRepresentation→ParamUnivElt R)

  -- -- -- PshFunctorRepresentation → ParamUniversalElement
  -- -- PshFunctorRepresentation→ParamUniversalElement : PshFunctorRepresentation →
  -- --                                                  ParamUniversalElement
  -- -- PshFunctorRepresentation→ParamUniversalElement R =
  -- --   ParamUnivElt→ParamUniversalElement (PshFunctorRepresentation→ParamUnivElt R)

  -- -- -- ParamUnivElt → ProfRepresentation
  -- -- ParamUnivElt→ProfRepresentation : ParamUnivElt → ProfRepresentation
  -- -- ParamUnivElt→ProfRepresentation U =
  -- --   PshFunctorRepresentation→ProfRepresentation
  -- --     (ParamUnivElt→PshFunctorRepresentation U)

  -- -- -- ParamUniversalElement → ProfRepresentation
  -- -- ParamUniversalElement→ProfRepresentation : ParamUniversalElement →
  -- --                                            ProfRepresentation
  -- -- ParamUniversalElement→ProfRepresentation U =
  -- --   ParamUnivElt→ProfRepresentation (ParamUniversalElement→ParamUnivElt U)

  -- -- -- ParamUniversalElement → PshFunctorRepresentation
  -- -- ParamUniversalElement→PshFunctorRepresentation : ParamUniversalElement →
  -- --                                                  PshFunctorRepresentation
  -- -- ParamUniversalElement→PshFunctorRepresentation U =
  -- --   ParamUnivElt→PshFunctorRepresentation (ParamUniversalElement→ParamUnivElt U)
